code/streaming/Hacl.Streaming.Interface.fsti
@@ -25,28 +25,104 @@ let uint8 = Lib.IntTypes.uint8
 inline_for_extraction noextract
 let uint32 = Lib.IntTypes.uint32
 
-/// The type class of block-based operations.
-/// Equipped with a generic index. May be unit if there's no agility, or hash algorithm for agility.
+/// The type class of stateful types.
+/// Needs to obey framing principles. Standard notion of footprint & invariant.
+inline_for_extraction noextract noeq
+type stateful (index: Type0) =
+| Stateful:
+  // Low-level types
+  s: (index -> Type0) ->
+
+  // Astract footprint.
+  footprint: (#i:index -> h:HS.mem -> s:s i -> GTot B.loc) ->
+  freeable: (#i:index -> h:HS.mem -> p:s i -> Type) ->
+  invariant: (#i:index -> h:HS.mem -> s:s i -> Type) ->
+
+  // A pure representation of a s
+  t: (index -> Type0) ->
+  v: (i:index -> h:HS.mem -> s:s i -> GTot (t i)) ->
+
+  // Adequate framing lemmas, relying on v.
+  invariant_loc_in_footprint: (#i:index -> h:HS.mem -> s:s i -> Lemma
+    (requires (invariant h s))
+    (ensures (B.loc_in (footprint #i h s) h))
+    [ SMTPat (invariant h s) ]) ->
+
+  frame_invariant: (#i:index -> l:B.loc -> s:s i -> h0:HS.mem -> h1:HS.mem -> Lemma
+    (requires (
+      invariant h0 s /\
+      B.loc_disjoint l (footprint #i h0 s) /\
+      B.modifies l h0 h1))
+    (ensures (
+      invariant h1 s /\
+      v i h0 s == v i h1 s /\
+      footprint #i h1 s == footprint #i h0 s))) ->
+
+  frame_freeable: (#i:index -> l:B.loc -> s:s i -> h0:HS.mem -> h1:HS.mem -> Lemma
+    (requires (
+      invariant h0 s /\
+      freeable h0 s /\
+      B.loc_disjoint l (footprint #i h0 s) /\
+      B.modifies l h0 h1))
+    (ensures (
+      freeable h1 s))
+    [ SMTPat (freeable h1 s); SMTPat (B.modifies l h0 h1) ]) ->
+
+  stateful index
+
+inline_for_extraction noextract
+let stateful_buffer (a: Type) (l: nat): stateful unit =
+  Stateful
+    (fun _ -> b:B.buffer a { B.length b == l })
+    (fun #_ h s -> B.loc_addr_of_buffer s)
+    (fun #_ h s -> B.freeable s)
+    (fun #_ h s -> B.live h s)
+    (fun _ -> s:S.seq a { S.length s == l })
+    (fun _ h s -> B.as_seq h s)
+    (fun #_ h s -> ())
+    (fun #_ l s h0 h1 -> ())
+    (fun #_ l s h0 h1 -> ())
+
+inline_for_extraction noextract
+let stateful_unused: stateful unit =
+  Stateful
+    (fun _ -> unit)
+    (fun #_ h s -> B.loc_none)
+    (fun #_ h s -> True)
+    (fun #_ h s -> True)
+    (fun _ -> unit)
+    (fun _ h s -> ())
+    (fun #_ h s -> ())
+    (fun #_ l s h0 h1 -> ())
+    (fun #_ l s h0 h1 -> ())
+
+type key_management =
+  | None
+  | Init
+  | InitFinish
+
+/// The type class of block-based operations. Equipped with a generic index. May
+/// be unit if there's no agility, or hash algorithm for agility.
+///
+/// The first index determines the role of the key:
+///
+/// - None: no key is used by this algorithm (e.g. hash)
+/// - Init: a key is needed at initialization-time (e.g. blake2, keyed hash
+///   functionality). Implementation retains a ghost key.
+/// - InitFinish: a key is needed at initialization-time and at the end of
+///   processing (e.g. poly1305). Implementation retains key at run-time.
+///
+/// Two things to note. First, we could always do the latter but this would
+/// retain useless state in the first two cases. Second, this distinction is
+/// only relevant for low-level functions, as spec functions just need to ignore
+/// their arguments.
 inline_for_extraction noextract noeq
 type block (index: Type0) =
 | Block:
 
-  // Astract footprint.
-  state: (index -> Type0) ->
-  footprint: (#i:index -> h:HS.mem -> s:state i -> GTot B.loc) ->
-
-  freeable: (#i:index -> h:HS.mem -> p:state i -> Type) ->
-  invariant: (#i:index -> h:HS.mem -> s:state i -> Type) ->
-
-  index_of_state: (i:G.erased index -> (
-    let i = G.reveal i in
-    s: state i -> Stack index
-    (fun h0 -> invariant h0 s)
-    (fun h0 i' h1 -> h0 == h1 /\ i' == i))) ->
-
-  // A pure representation of a state
-  t: (index -> Type0) ->
-  v: (#i:index -> h:HS.mem -> s:state i -> GTot (t i)) ->
+  // Low-level types
+  state: stateful index ->
+  key: stateful index ->
 
   // Introducing a notion of blocks and final result.
   max_input_length: (index -> x:nat { 0 < x /\ x < pow2 64 }) ->
@@ -55,26 +131,26 @@ type block (index: Type0) =
 
   /// An init/update/update_last/finish specification. The long refinements were
   /// previously defined as blocks / small / output.
-  init_s: (i:index -> t i) ->
-  update_multi_s: (i:index -> t i -> s:S.seq uint8 { S.length s % U32.v (block_len i) = 0 } -> t i) ->
+  init_s: (i:index -> key.t i -> state.t i) ->
+  update_multi_s: (i:index -> state.t i -> s:S.seq uint8 { S.length s % U32.v (block_len i) = 0 } -> state.t i) ->
   update_last_s: (i:index ->
-    t i ->
+    state.t i ->
     prevlen:nat { prevlen % U32.v (block_len i) = 0 } ->
-    s:S.seq uint8 { S.length s + prevlen <= max_input_length i } ->
-    t i) ->
-  finish_s: (i:index -> t i -> s:S.seq uint8 { S.length s = U32.v (output_len i) }) ->
+    s:S.seq uint8 { S.length s + prevlen <= max_input_length i /\ S.length s < U32.v (block_len i) } ->
+    state.t i) ->
+  finish_s: (i:index -> key.t i -> state.t i -> s:S.seq uint8 { S.length s = U32.v (output_len i) }) ->
 
   /// The specification in one shot.
-  spec_s: (i:index -> input:S.seq uint8 { S.length input <= max_input_length i } ->
+  spec_s: (i:index -> key.t i -> input:S.seq uint8 { S.length input <= max_input_length i } ->
     output:S.seq uint8 { S.length output == U32.v (output_len i) }) ->
 
   // Required lemmas... clients can enjoy them in their local contexts with the SMT pattern via a let-binding.
 
-  update_multi_zero: (i:index -> h:t i -> Lemma
+  update_multi_zero: (i:index -> h:state.t i -> Lemma
     (ensures (update_multi_s i h S.empty == h))) ->
 
   update_multi_associative: (i:index ->
-    h: t i ->
+    h: state.t i ->
     input1:S.seq uint8 ->
     input2:S.seq uint8 ->
     Lemma
@@ -89,6 +165,7 @@ type block (index: Type0) =
     [ SMTPat (update_multi_s i (update_multi_s i h input1) input2) ]) ->
 
   spec_is_incremental: (i:index ->
+    key: key.t i ->
     input:S.seq uint8 { S.length input <= max_input_length i } ->
     Lemma (ensures (
       let open FStar.Mul in
@@ -96,145 +173,133 @@ type block (index: Type0) =
       let n = S.length input / block_length in
       let bs, l = S.split input (n * block_length) in
       FStar.Math.Lemmas.multiple_modulo_lemma n block_length;
-      let hash = update_multi_s i (init_s i) bs in
+      let hash = update_multi_s i (init_s i key) bs in
       let hash = update_last_s i hash (n * block_length) l in
-      finish_s i hash `S.equal` spec_s i input))) ->
-
-  // Adequate framing lemmas
-  invariant_loc_in_footprint: (#i:index -> h:HS.mem -> s:state i -> Lemma
-    (requires (invariant h s))
-    (ensures (B.loc_in (footprint #i h s) h))
-    [ SMTPat (invariant h s) ]) ->
-
-  frame_invariant: (#i:index -> l:B.loc -> s:state i -> h0:HS.mem -> h1:HS.mem -> Lemma
-    (requires (
-      invariant h0 s /\
-      B.loc_disjoint l (footprint #i h0 s) /\
-      B.modifies l h0 h1))
-    (ensures (
-      invariant h1 s /\
-      v h0 s == v h1 s /\
-      footprint #i h1 s == footprint #i h0 s))) ->
-
-  frame_freeable: (#i:index -> l:B.loc -> s:state i -> h0:HS.mem -> h1:HS.mem -> Lemma
-    (requires (
-      invariant h0 s /\
-      freeable h0 s /\
-      B.loc_disjoint l (footprint #i h0 s) /\
-      B.modifies l h0 h1))
-    (ensures (
-      freeable h1 s))
-    [ SMTPat (freeable h1 s); SMTPat (B.modifies l h0 h1) ]) ->
+      finish_s i key hash `S.equal` spec_s i key input))) ->
 
   // Stateful operations
-  alloca: (i:index -> StackInline (state i)
+  index_of_state: (i:G.erased index -> (
+    let i = G.reveal i in
+    s: state.s i -> Stack index
+    (fun h0 -> state.invariant #i h0 s)
+    (fun h0 i' h1 -> h0 == h1 /\ i' == i))) ->
+
+  alloca: (i:index -> StackInline (state.s i)
     (requires (fun _ -> True))
     (ensures (fun h0 s h1 ->
-      invariant h1 s /\
+      state.invariant #i h1 s /\
       B.(modifies loc_none h0 h1) /\
-      B.fresh_loc (footprint #i h1 s) h0 h1 /\
-      B.(loc_includes (loc_region_only true (HS.get_tip h1)) (footprint #i h1 s))))) ->
+      B.fresh_loc (state.footprint #i h1 s) h0 h1 /\
+      B.(loc_includes (loc_region_only true (HS.get_tip h1)) (state.footprint #i h1 s))))) ->
 
-  create_in: (i:index -> r:HS.rid -> ST (state i)
-    (requires (fun _ ->
+  create_in: (i:index ->
+    r:HS.rid ->
+    ST (state.s i)
+    (requires (fun h0 ->
       HyperStack.ST.is_eternal_region r))
     (ensures (fun h0 s h1 ->
-      invariant h1 s /\
+      state.invariant #i h1 s /\
       B.(modifies loc_none h0 h1) /\
-      B.fresh_loc (footprint #i h1 s) h0 h1 /\
-      B.(loc_includes (loc_region_only true r) (footprint #i h1 s)) /\
-      freeable h1 s))) ->
+      B.fresh_loc (state.footprint #i h1 s) h0 h1 /\
+      B.(loc_includes (loc_region_only true r) (state.footprint #i h1 s)) /\
+      state.freeable #i h1 s))) ->
 
   init: (i:G.erased index -> (
     let i = G.reveal i in
-    s: state i -> Stack unit
-    (requires fun h0 -> invariant #i h0 s)
+    k: key.s i ->
+    s: state.s i -> Stack unit
+    (requires fun h0 ->
+      key.invariant #i h0 k /\
+      state.invariant #i h0 s /\
+      B.loc_disjoint (key.footprint #i h0 k) (state.footprint #i h0 s))
     (ensures fun h0 _ h1 ->
-      invariant #i h1 s /\
-      v h1 s == init_s i /\
-      B.(modifies (footprint #i h0 s) h0 h1) /\
-      footprint #i h0 s == footprint #i h1 s /\
-      (freeable h0 s ==> freeable h1 s)))) ->
+      key.invariant #i h1 k /\
+      (key.freeable #i h0 k ==> key.freeable #i h1 k) /\
+      state.invariant #i h1 s /\
+      state.v i h1 s == init_s i (key.v i h0 k) /\
+      B.(modifies (state.footprint #i h0 s) h0 h1) /\
+      state.footprint #i h0 s == state.footprint #i h1 s /\
+      (state.freeable #i h0 s ==> state.freeable #i h1 s)))) ->
 
   update_multi: (i:G.erased index -> (
     let i = G.reveal i in
-    s:state i ->
+    s:state.s i ->
     blocks:B.buffer uint8 { B.length blocks % U32.v (block_len i) = 0 } ->
     len: U32.t { U32.v len = B.length blocks } ->
     Stack unit
     (requires fun h0 ->
-      invariant #i h0 s /\
+      state.invariant #i h0 s /\
       B.live h0 blocks /\
-      B.(loc_disjoint (footprint #i h0 s) (loc_buffer blocks)))
+      B.(loc_disjoint (state.footprint #i h0 s) (loc_buffer blocks)))
     (ensures fun h0 _ h1 ->
-      B.(modifies (footprint #i h0 s) h0 h1) /\
-      footprint #i h0 s == footprint #i h1 s /\
-      invariant #i h1 s /\
-      v h1 s == update_multi_s i (v h0 s) (B.as_seq h0 blocks) /\
-      (freeable #i h0 s ==> freeable #i h1 s)))) ->
+      B.(modifies (state.footprint #i h0 s) h0 h1) /\
+      state.footprint #i h0 s == state.footprint #i h1 s /\
+      state.invariant #i h1 s /\
+      state.v i h1 s == update_multi_s i (state.v i h0 s) (B.as_seq h0 blocks) /\
+      (state.freeable #i h0 s ==> state.freeable #i h1 s)))) ->
 
   update_last: (
     i: G.erased index -> (
     let i = G.reveal i in
-    s:state i ->
+    s:state.s i ->
     last:B.buffer uint8 { B.len last < block_len i } ->
     total_len:U64.t {
       U64.v total_len <= max_input_length i /\
       (U64.v total_len - B.length last) % U32.v (block_len i) = 0 } ->
     Stack unit
     (requires fun h0 ->
-      invariant #i h0 s /\
+      state.invariant #i h0 s /\
       B.live h0 last /\
-      B.(loc_disjoint (footprint #i h0 s) (loc_buffer last)))
+      B.(loc_disjoint (state.footprint #i h0 s) (loc_buffer last)))
     (ensures fun h0 _ h1 ->
-      invariant #i h1 s /\
-      v h1 s == update_last_s i (v h0 s) (U64.v total_len - B.length last) (B.as_seq h0 last) /\
-      B.(modifies (footprint #i h0 s) h0 h1) /\
-      footprint #i h0 s == footprint #i h1 s /\
-      (freeable #i h0 s ==> freeable #i h1 s)))) ->
+      state.invariant #i h1 s /\
+      state.v i h1 s == update_last_s i (state.v i h0 s) (U64.v total_len - B.length last) (B.as_seq h0 last) /\
+      B.(modifies (state.footprint #i h0 s) h0 h1) /\
+      state.footprint #i h0 s == state.footprint #i h1 s /\
+      (state.freeable #i h0 s ==> state.freeable #i h1 s)))) ->
 
   finish: (
     i: G.erased index -> (
     let i = G.reveal i in
-    s:state i ->
+    s:state.s i ->
     dst:B.buffer uint8 { B.len dst = output_len i } ->
     Stack unit
     (requires fun h0 ->
-      invariant #i h0 s /\
+      state.invariant #i h0 s /\
       B.live h0 dst /\
-      B.(loc_disjoint (footprint #i h0 s) (loc_buffer dst)))
+      B.(loc_disjoint (state.footprint #i h0 s) (loc_buffer dst)))
     (ensures fun h0 _ h1 ->
-      invariant #i h1 s /\
+      state.invariant #i h1 s /\
       B.(modifies (loc_buffer dst) h0 h1) /\
-      footprint #i h0 s == footprint #i h1 s /\
-      B.as_seq h1 dst == finish_s i (v h0 s) /\
-      (freeable #i h0 s ==> freeable #i h1 s)))) ->
+      state.footprint #i h0 s == state.footprint #i h1 s /\
+      B.as_seq h1 dst == finish_s i (state.v i h0 s) /\
+      (state.freeable #i h0 s ==> state.freeable #i h1 s)))) ->
 
   free: (
     i: G.erased index -> (
     let i = G.reveal i in
-    s:state i -> ST unit
+    s:state.s i -> ST unit
     (requires fun h0 ->
-      freeable h0 s /\
-      invariant #i h0 s)
+      state.freeable #i h0 s /\
+      state.invariant #i h0 s)
     (ensures fun h0 _ h1 ->
-      B.(modifies (footprint #i h0 s) h0 h1)))) ->
+      B.(modifies (state.footprint #i h0 s) h0 h1)))) ->
 
   copy: (
     i:G.erased index -> (
     let i = G.reveal i in
-    s_src:state i ->
-    s_dst:state i ->
+    s_src:state.s i ->
+    s_dst:state.s i ->
     Stack unit
       (requires (fun h0 ->
-        invariant #i h0 s_src /\
-        invariant #i h0 s_dst /\
-        B.(loc_disjoint (footprint #i h0 s_src) (footprint #i h0 s_dst))))
+        state.invariant #i h0 s_src /\
+        state.invariant #i h0 s_dst /\
+        B.(loc_disjoint (state.footprint #i h0 s_src) (state.footprint #i h0 s_dst))))
       (ensures fun h0 _ h1 ->
-        B.(modifies (footprint #i h0 s_dst) h0 h1) /\
-        footprint #i h0 s_dst == footprint #i h1 s_dst /\
-        (freeable h0 s_dst ==> freeable h1 s_dst) /\
-        invariant #i h1 s_dst /\
-        v h1 s_dst == v h0 s_src))) ->
+        B.(modifies (state.footprint #i h0 s_dst) h0 h1) /\
+        state.footprint #i h0 s_dst == state.footprint #i h1 s_dst /\
+        (state.freeable #i h0 s_dst ==> state.freeable #i h1 s_dst) /\
+        state.invariant #i h1 s_dst /\
+        state.v i h1 s_dst == state.v i h0 s_src))) ->
 
   block index
